jump_serializer, list_last_pos, parse_truncate
Imported from project-everest/mitls-fstar@179421862c7290b2b540c954807bfae32af31682

src/lowparse/LowParse.Low.Base.fst
@@ -2086,6 +2086,61 @@ let jump_constant_size
   [@inline_let] let _ = valid_facts p h input pos in
   pos `U32.add` sz
 
+let seq_starts_with (#t: Type) (slong sshort: Seq.seq t) : GTot Type0 =
+  Seq.length sshort <= Seq.length slong /\
+  Seq.slice slong 0 (Seq.length sshort) `Seq.equal` sshort
+
+let seq_starts_with_trans (#t: Type) (s1 s2 s3: Seq.seq t) : Lemma
+  (requires (s1 `seq_starts_with` s2 /\ s2 `seq_starts_with` s3))
+  (ensures (s1 `seq_starts_with` s3))
+= ()
+
+let seq_starts_with_append_l_intro (#t: Type) (s1 s2: Seq.seq t) : Lemma
+  ((s1 `Seq.append` s2) `seq_starts_with` s1)
+= ()
+
+let seq_starts_with_append_r_elim (#t: Type) (s s1 s2: Seq.seq t) : Lemma
+  (requires (s `seq_starts_with` (s1 `Seq.append` s2)))
+  (ensures (
+    s `seq_starts_with` s1 /\
+    Seq.slice s (Seq.length s1) (Seq.length s) `seq_starts_with` s2
+  ))
+  [SMTPat (s `seq_starts_with` (s1 `Seq.append` s2))]
+= let s3 = Seq.slice s (Seq.length s1 + Seq.length s2) (Seq.length s) in
+  assert (s `Seq.equal` (s1 `Seq.append` s2 `Seq.append` s3))
+
+inline_for_extraction
+noextract
+let jump_serializer
+  (#k: _)
+  (#t: _)
+  (#p: parser k t)
+  (s: serializer p { k.parser_kind_subkind == Some ParserStrong })
+  (j: jumper p)
+  (#rrel #rel: _)
+  (sl: slice rrel rel)
+  (pos: U32.t)
+  (x: Ghost.erased t)
+: HST.Stack U32.t
+  (requires (fun h ->
+    let sq = serialize s (Ghost.reveal x) in
+    live_slice h sl /\
+    U32.v pos <= U32.v sl.len /\
+    bytes_of_slice_from h sl pos `seq_starts_with` sq
+  ))
+  (ensures (fun h res h' ->
+    B.modifies B.loc_none h h' /\
+    U32.v pos + Seq.length (serialize s (Ghost.reveal x)) == U32.v res
+  ))
+= let h = HST.get () in
+  let gsq = Ghost.hide (serialize s (Ghost.reveal x)) in
+  let glen = Ghost.hide (Seq.length (Ghost.reveal gsq)) in
+  let gpos' = Ghost.hide (pos `U32.add` U32.uint_to_t (Ghost.reveal glen)) in
+  assert (bytes_of_slice_from_to h sl pos (Ghost.reveal gpos') == Seq.slice (bytes_of_slice_from h sl pos) 0 (Seq.length (serialize s (Ghost.reveal x))));
+  serialize_valid_exact s h sl (Ghost.reveal x) pos (Ghost.reveal gpos');
+  valid_exact_valid p h sl pos (Ghost.reveal gpos');
+  j sl pos
+
 [@unifier_hint_injective]
 inline_for_extraction
 let leaf_reader
