src/lowparse/LowParse.SLow.VCList.fst
@@ -217,7 +217,7 @@ let serialize32_nlist
 
 #pop-options
 
-#push-options "--z3rlimit 32"
+#push-options "--z3rlimit 64"
 
 inline_for_extraction
 let size32_nlist
